some more work on the subgraph time black hole

Kura/Graph/Subgraph.lean
@@ -27,7 +27,7 @@ structure QuotientSubgraph (G : Graph V E) where
   vmap'_idem : ∀ v, Option.bind (vmap' v) vmap' = vmap' v
   Eset : Set E
   DecEMem : DecidablePred (· ∈ Eset)
-  Eset_spec : ∀ e v, vmap' v = ⊥ → v ∈ G.inc e → e ∉ Eset
+  Eset_spec : ∀ e ∈ Eset, ∀ v ∈ G.inc e, (vmap' v).isSome
 
 ----------------------------------------------------------------------
 -- useful lemma
@@ -41,6 +41,13 @@ lemma Subgraph.not_mem_Eset  (S : Subgraph G) (he : ∃ v ∈ G.inc e, v ∉ S.V
   push_neg
   exact he
 
+lemma QuotientSubgraph.not_mem_Eset (S : QuotientSubgraph G) (he : ∃ v ∈ G.inc e, (S.vmap' v).isNone) :
+    e ∉ S.Eset := by
+  intro h
+  absurd S.Eset_spec e h
+  push_neg
+  simpa only [ne_eq, Bool.not_eq_true, Option.not_isSome, Option.isNone_iff_eq_none] using he
+
 /-- Expose the decidability of (· ∈ Vset) -/
 instance InducedSubgraphDecVMem {G : Graph V E} (S : InducedSubgraph G) :
     DecidablePred (· ∈ S.Vset) := S.DecVMem
@@ -53,6 +60,22 @@ instance SubgraphDecEMem (S : Subgraph G) : DecidablePred (· ∈ S.Eset) := S.D
 lemma QuotientGraph.vmap_idem_for_simp  (S : QuotientGraph G) (v : V) :
     S.vmap (S.vmap v) = S.vmap v := S.vmap_idem v
 
+/-- Expose the decidability of (· ∈ Eset)-/
+instance QuotientSubgraphDecEMem (S : QuotientSubgraph G) : DecidablePred (· ∈ S.Eset) := S.DecEMem
+
+-------------------------------------------------
+-- Evaluations
+
+def InducedSubgraph.eval (S : InducedSubgraph G) :
+  Graph S.Vset {e // (G.inc e).all (· ∈ S.Vset) } where
+  inc e := edge.pmap Subtype.mk (G.inc e.1) (by
+    simpa only [all_iff, decide_eq_true_eq] using e.prop)
+
+def Subgraph.eval (S : Subgraph G) :
+  Graph S.Vset S.Eset where
+  inc e := edge.pmap Subtype.mk (G.inc e.1) (S.Eset_spec e.val e.prop)
+
+-- some setup is needed to make this work for QuotientGraph
 def QuotientGraph.ran (S : QuotientGraph G) : Set V :=
   {v | ∃ u, S.vmap u = v}
 
@@ -70,27 +93,37 @@ lemma QuotientGraph.mem_ran_iff_vmap_self (S : QuotientGraph G) (v : V) :
   · rintro h
     exact ⟨ v, h ⟩
 
-def QuotientGraph.vmap' (S : QuotientGraph G) (v : V) : S.ran :=
+def QuotientGraph.vmapRan (S : QuotientGraph G) (v : V) : S.ran :=
   ⟨ S.vmap v, by rw [mem_ran_iff_vmap_self, vmap_idem_for_simp]⟩
 
+def QuotientGraph.eval (S : QuotientGraph G) : Graph (S.ran) E where
+  inc e := (G.inc e).map S.vmapRan
+
+-- Even more setup is needed to make this work for QuotientSubgraph
 def QuotientSubgraph.ran (S : QuotientSubgraph G) : Set V :=
   {v | ∃ u, S.vmap' u = some v}
 
+def QuotientSubgraph.Vset (S : QuotientSubgraph G) : Set V :=
+  {v | (S.vmap' v).isSome }
 
--------------------------------------------------
--- Evaluations
+@[simp]
+lemma QuotientSubgraph.mem_Vset_iff (S : QuotientSubgraph G) (v : V) :
+    v ∈ S.Vset ↔ (S.vmap' v).isSome := Iff.rfl
 
-def InducedSubgraph.eval (S : InducedSubgraph G) :
-  Graph S.Vset {e // (G.inc e).all (· ∈ S.Vset) } where
-  inc e := edge.pmap Subtype.mk (G.inc e.1) (by
-    simpa only [all_iff, decide_eq_true_eq] using e.prop)
+/-- if e is in Eset, all vertices incident to e is not removed.
+  Embed this fact to the type of each v. -/
+def QuotientSubgraph.domSubtype (S : QuotientSubgraph G) (e : S.Eset) : edge S.Vset :=
+  (G.inc e).pmap Subtype.mk (fun v hv => S.Eset_spec e.val e.prop v hv)
 
-def Subgraph.eval (S : Subgraph G) :
-  Graph S.Vset S.Eset where
-  inc e := edge.pmap Subtype.mk (G.inc e.1) (S.Eset_spec e.val e.prop)
+def QuotientSubgraph.vmap'Ran (S : QuotientSubgraph G) (v : S.Vset) : S.ran :=
+  ⟨ (S.vmap' v.val).get v.prop, by simp only [ran, Set.mem_setOf_eq, Option.some_get,
+    exists_apply_eq_apply]⟩
 
-def QuotientGraph.eval (S : QuotientGraph G) : Graph (S.ran) E where
-  inc e := (G.inc e).map S.vmap'
+def QuotientSubgraph.eval (S : QuotientSubgraph G) : Graph S.ran S.Eset where
+  inc e := S.domSubtype e |>.map S.vmap'Ran
+
+------------------------------------------------------------------------
+-- Carrying over the instances
 
 instance InducedSubgraphFullgraph [fullGraph G] (S : InducedSubgraph G) :
   fullGraph (V := S.Vset) S.eval where
@@ -98,6 +131,14 @@ instance InducedSubgraphFullgraph [fullGraph G] (S : InducedSubgraph G) :
 
 instance SubgraphFullgraph [fullGraph G] (S : Subgraph G) :
   fullGraph (V := S.Vset) S.eval where
+  all_full := sorry
+
+instance QuotientGraphFullgraph [fullGraph G] (S : QuotientGraph G) :
+  fullGraph (V := S.ran) S.eval where
+  all_full := sorry
+
+instance QuotientSubgraphFullgraph [fullGraph G] (S : QuotientSubgraph G) :
+  fullGraph (V := S.ran) S.eval where
   all_full := sorry
 
 instance InducedSubgraphUndirected [Undirected G] (S : InducedSubgraph G) :
@@ -108,6 +149,13 @@ instance SubgraphUndirected [Undirected G] (S : Subgraph G) :
   Undirected (V := S.Vset) S.eval where
   edge_symm := sorry
 
+instance QuotientGraphUndirected [Undirected G] (S : QuotientGraph G) :
+  Undirected (V := S.ran) S.eval where
+  edge_symm := sorry
+
+instance QuotientSubgraphUndirected [Undirected G] (S : QuotientSubgraph G) :
+  Undirected (V := S.ran) S.eval where
+  edge_symm := sorry
 
 -----------------------------------------------------------------------------
 -- Initializations
@@ -134,8 +182,7 @@ def QuotientSubgraph.init : QuotientSubgraph G where
   vmap'_idem := by simp only [Option.bind_some, implies_true]
   Eset := Set.univ
   DecEMem := by infer_instance
-  Eset_spec := by simp only [reduceCtorEq, Set.mem_univ, not_true_eq_false, imp_false,
-    false_implies, implies_true]
+  Eset_spec := by simp only [Set.mem_univ, Option.isSome_some, implies_true, imp_self]
 
 -----------------------------------------------------------------------------
 -- Elementary operations
@@ -151,7 +198,7 @@ def InducedSubgraph.OnSet (G' : InducedSubgraph G) (S : Set V) [DecidablePred (�
   Vset := G'.Vset ∩ S
   DecVMem := by infer_instance
 
-macro G:term "[" S:term "]" : term =>
+macro G:term "[" S:term "]ᴳ" : term =>
   `(InducedSubgraph.eval (InducedSubgraph.OnSet (InducedSubgraph.init $G) $S))
 
 
@@ -196,7 +243,7 @@ def Subgraph.OnSetE (G' : Subgraph G) (S : Set E) [DecidablePred (· ∈ S)] : S
     simp only [Set.mem_inter_iff] at he
     exact G'.Eset_spec e he.1 u hu
 
-macro G:term "{" S:term "}" : term => `(Subgraph.eval (Subgraph.OnSetE (Subgraph.init $G) $S))
+macro G:term "{" S:term "}ᴳ" : term => `(Subgraph.eval (Subgraph.OnSetE (Subgraph.init $G) $S))
 
 /-- The second vertex is being merged into the first vertex-/
 def QuotientGraph.merge (G' : QuotientGraph G) (v w : V) :
@@ -210,6 +257,26 @@ def QuotientGraph.mergeOnSet (G' : QuotientGraph G) (S : Set V) [DecidablePred (
   vmap u := if G'.vmap u ∈ S then G'.vmap x else G'.vmap u
   vmap_idem u := by
     by_cases hu : G'.vmap u ∈ S <;> simp only [hu, ↓reduceIte, vmap_idem_for_simp, ite_self]
+
+
+def QuotientSubgraph.vrm [DecidableEq E] (G' : QuotientSubgraph G) (v : V) :
+    QuotientSubgraph G where
+  vmap' u := if G'.vmap' u = v then ⊥ else G'.vmap' u
+  vmap'_idem u := by
+    by_cases hu : G'.vmap' u = v <;> simp [hu, ↓reduceIte]
+    · rfl
+    · by_cases hvu : (G'.vmap' u) = none
+      · simp only [hvu, Option.none_bind]
+      · obtain ⟨w, hw⟩ := Option.ne_none_iff_exists.mp hvu
+        simp only [← hw, Option.some_bind]
+        sorry
+  Eset := {e ∈ G'.Eset | G.all e (G'.vmap' · ≠ v)}
+  DecEMem := by infer_instance
+  Eset_spec e he u hu := by
+    simp only [ne_eq, decide_not, all_iff, Bool.not_eq_true', decide_eq_false_iff_not,
+      Set.mem_setOf_eq] at he
+    simp only [he.2 u hu, ↓reduceIte]
+    exact G'.Eset_spec e he.1 u hu
 
 ------------------------------------------------------------------------
 -- Lemmas about the elementary operations
